

$$2(3) f = \ln(x^2 + y) \text{ в } (0; 1)$$

$$\frac{\partial f}{\partial x} = \frac{2x}{x^2 + y}; \frac{\partial f}{\partial y} = \frac{1}{x^2 + y} - \text{непрерывны в окр-ти } (0; 1) \Rightarrow \frac{\partial^2 f}{\partial x \partial y} = \frac{\partial^2 f}{\partial y \partial x}$$

$$\frac{\partial^2 f}{\partial x \partial y}(0; 1) = \frac{\partial}{\partial y} \left( \frac{\partial f}{\partial x} \right) = \frac{-x^2 \cdot 2x}{(x^2 + y)^2} (0; 1) = 0 = \frac{\partial^2 f}{\partial y \partial x}$$

$$\frac{\partial^2 f}{\partial x^2}(0; 1) = \frac{\partial}{\partial x} \left( \frac{\partial f}{\partial x} \right) \Big|_{(0; 1)} = \frac{2(x^2 + y) - 2x \cdot 2x}{(x^2 + y)^2} \Big|_{(0; 1)} = \frac{2y - 2x^2}{(x^2 + y^2)^2} \Big|_{(0; 1)} = 2$$

$$\frac{\partial^2 f}{\partial y^2}(0; 1) = \frac{\partial}{\partial y} \left( \frac{\partial f}{\partial y} \right) \Big|_{(0; 1)} = -\frac{1}{(x^2 + y)^3} \Big|_{(0; 1)} = -1$$

$$d^2 f = 2dx^2 - dy^2$$

$$4. f = \begin{cases} xy(x^2 - y^2)/(x^2 + y^2), & x^2 + y^2 \neq 0 \\ 0, & x^2 + y^2 = 0 \end{cases}$$

$$\frac{\partial f}{\partial x} = \left( \frac{xy(x^2 - y^2)}{x^2 + y^2} \right)'_x = \frac{(3yx^2 - y^3)(x^2 + y^2) - 2x^2y(x^2 - y^2)}{(x^2 + y^2)^2} = \frac{x^4y + 4x^2y^3 - y^5}{(x^2 + y^2)^2}$$

$$\frac{\partial f}{\partial x}(0; 0) = \lim_{x \rightarrow 0} \frac{f(x, 0) - f(0, 0)}{x} = 0$$

$$\frac{\partial f}{\partial y} = \frac{x^5 - y^4x - 4y^2x^3}{(x^2 + y^2)^2} \text{ (симметрично } \frac{\partial f}{\partial x}, \text{ но с минусом)}$$

$$\frac{\partial f}{\partial y}(0; 0) = \lim_{y \rightarrow 0} \frac{f(0, y) - f(0, 0)}{y} = 0$$

$$\frac{\partial^2 f}{\partial x \partial y}(0; 0) = \frac{\partial}{\partial y} \left( \frac{\partial f}{\partial x} \right) \Big|_{(0; 0)} = \lim_{y \rightarrow 0} \frac{\frac{\partial f}{\partial x}(0; y) - \frac{\partial f}{\partial x}(0; 0)}{y} = \lim_{y \rightarrow 0} \frac{-y^5}{y^5} = -1$$

$$\frac{\partial^2 f}{\partial y \partial x}(0; 0) = \frac{\partial}{\partial x} \left( \frac{\partial f}{\partial y} \right) \Big|_{(0; 0)} = \lim_{x \rightarrow 0} \frac{\frac{\partial f}{\partial y}(x; 0) - \frac{\partial f}{\partial y}(0; 0)}{x} = \lim_{x \rightarrow 0} \frac{x^5}{x^5} = 1$$

$$15(2) f = e^{x^2/y} \text{ в т. } (1; 1)$$

$$\frac{\partial f}{\partial x} = e^{x^2/y} \cdot \frac{2x}{y}; \frac{\partial f}{\partial y} = e^{x^2/y} \left( -\frac{x^2}{y^2} \right) - \text{непр. в окр-ти } (1; 1) \Rightarrow \frac{\partial^2 f}{\partial x \partial y} = \frac{\partial^2 f}{\partial y \partial x}$$

$$\frac{\partial^2 f}{\partial x^2}(1; 1) = \left( e^{\frac{x^2}{y}} \cdot \frac{4x^2}{y^2} + \frac{2}{y} e^{\frac{x^2}{y}} \right) \Big|_{(1; 1)} = 6e$$

$$\frac{\partial^2 f}{\partial x \partial y}(1; 1) = \frac{\partial}{\partial y} \left( \frac{\partial f}{\partial x} \right) (1; 1) = \left( e^{\frac{x^2}{y}} \left( -\frac{x^2}{y^2} \cdot \frac{2x}{y} \right) - \frac{2x}{y^2} e^{\frac{x^2}{y}} \right) \Big|_{(1; 1)} = -4e$$

$$\frac{\partial^2 f}{\partial y^2}(1;1) = \left( e^{x^2/y} \frac{x^4}{y^4} + \frac{2x^2}{y^3} e^{x^2/y} \right) \Big|_{(1;1)} = 3e$$

$$d^2 f = 6e dx^2 - 8e dx dy + 3e dy^2$$

$$71(2,4)$$

$$2) f(x,y) = \arctg \frac{1+x}{1+y} \text{ в окр-ти } (0;0)$$

$$\frac{\partial f}{\partial x} = \frac{1}{1 + \left(\frac{1+x}{1+y}\right)^2} \cdot \frac{1}{1+y} = \frac{1+y}{(1+y)^2 + (1+x)^2}; \quad \frac{\partial f}{\partial x}(0;0) = \frac{1}{2}$$

$$\frac{\partial f}{\partial y} = \frac{1}{1 + \left(\frac{1+x}{1+y}\right)^2} \cdot \left( -\frac{1+x}{(1+y)^2} \right) = \frac{-(1+x)}{(1+x)^2 + (1+y)^2}; \quad \frac{\partial f}{\partial y}(0;0) = -\frac{1}{2}$$

$$\frac{\partial^2 f}{\partial x^2} = -(1+y) \frac{2(1+x)}{((1+x)^2 + (1+y)^2)^2}; \quad \frac{\partial^2 f}{\partial x^2}(0;0) = -\frac{1}{2}$$

$$\frac{\partial^2 f}{\partial y^2} = (1+x) \frac{2(1+y)}{((1+x)^2 + (1+y)^2)^2}; \quad \frac{\partial^2 f}{\partial y^2}(0;0) = \frac{1}{2}$$

$$\frac{\partial^2 f}{\partial x \partial y} = \frac{(1+x)^2 + (1+y)^2 - 2(1+y)^2}{((1+x)^2 + (1+y)^2)^2}; \quad \frac{\partial^2 f}{\partial x \partial y}(0;0) = 0$$

$$f(x,y) = \frac{\pi}{4} + \frac{1}{2}x - \frac{1}{2}y + \frac{1}{2!} \left( -\frac{1}{2}x^2 + \frac{1}{2}y^2 \right) + \tilde{O}(\rho^2) = \frac{\pi}{4} + \frac{1}{2}x - \frac{1}{2}y - \frac{1}{4}x^2 + \frac{1}{4}y^2 + \tilde{O}(\rho^3), \rho \rightarrow 0$$

$$4) f(x,y) = \arctg(x^2 y - 2e^{x-1}) \text{ в окр-ти } (1;3)$$

$$\frac{\partial f}{\partial x}(1;3) = \frac{2xy - 2e^{x-1}}{1 + (x^2 y - 2e^{x-1})^2} = \frac{6-2}{2} = 2; \quad \frac{\partial f}{\partial y}(1;3) = \frac{x^2}{1 + (x^2 y - 2e^{x-1})^2} \Big|_{(1;3)} = \frac{1}{2}$$

$$\frac{\partial^2 f}{\partial x^2}(1;3) = \left( \frac{(2y - 2e^{x-1})(1 + (x^2 y - 2e^{x-1})^2) - 2(x^2 y - 2e^{x-1})(2xy - 2e^{x-1})}{(1 + (x^2 y - 2e^{x-1})^2)^2} \right) \Big|_{(1;3)} = -6$$

$$\frac{\partial^2 f}{\partial y^2}(1;3) = \frac{-x^2 \cdot x^2}{(1 + (x^2 y - 2e^{x-1})^2)^2} \cdot 2(x^2 y - 2e^{x-1}) = -\frac{1}{2}$$

$$\frac{\partial^2 f}{\partial x \partial y} = \frac{\partial^2 f}{\partial y \partial x} \left( \text{т.к. } \frac{\partial f}{\partial x}, \frac{\partial f}{\partial y} \text{ непрерывны в окр-ти } (1;3) \right) = \frac{\partial}{\partial x} \left( \frac{\partial f}{\partial y} \right) (1;3) =$$

$$= \frac{2x(1 + (x^2 y - 2e^{x-1})^2) - x^2 \cdot 2(x^2 y - 2e^{x-1})(2xy - 2e^{x-1})}{(1 + (x^2 y - 2e^{x-1})^2)^2} \Big|_{(1;3)} = -1$$

$$f(x, y) = \frac{\pi}{4} + 2(x-1) + \frac{1}{2}(y-3) + \frac{1}{2!} \left( -6(x-1)^2 - \frac{1}{6}(y-3)^2 - 2(x-1)(y-3) \right) + \dots$$

$$+ \tilde{O}(p^2) = \frac{\pi}{4} + 2(x-1) + \frac{1}{2}(y-3) - 3(x-1)^2 - \frac{1}{6}(y-3)^2 - (x-1)(y-3) + \tilde{O}(p^2),$$

$$p \rightarrow 0$$

$$74(4, 5) \partial_0 \tilde{O}(p^4)$$

$$4) f = \sin x / \cos y = \frac{x - \frac{x^3}{6} + \tilde{O}(x^4)}{1 - \frac{1}{2}y^2 + \tilde{O}(y^3)} = \left( x - \frac{1}{6}x^3 + \tilde{O}(x^4) \right) \left( 1 + \frac{1}{2}y^2 + \tilde{O}(y^3) \right) =$$

$$= 1 + \frac{1}{2}xy^2 - \frac{1}{6}x^3 + \tilde{O}(p^4), p \rightarrow 0$$

$$5) f = e^x \sin y = \left( 1 + x + \frac{1}{2}x^2 + \frac{1}{6}x^3 + \tilde{O}(x^3) \right) \left( y - \frac{1}{6}y^3 + \tilde{O}(y^4) \right) = y + xy - \frac{1}{6}y^3 + \frac{1}{2}x^2y - \frac{1}{6}xy^3 + \frac{1}{6}x^3y + \tilde{O}(p^4),$$

$$p \rightarrow 0$$

Донатик